VerificationCDPC.dfy
@@ -11,17 +11,14 @@ abstract module VerificationCDPC {
 method verifyCDPC
   (f:map<map<Question, Answer>, bool>, g:map<map<Question, Answer>, int>, P:set<Question>, k:int, a:real, b:real, Q:set<Question>, A:set<Answer>, interview:Interview)
   returns (R:bool)
-requires (forall m | m in f.Keys :: m.Keys == Q)
-requires (f.Keys == g.Keys)
-requires (P <= Q)
-requires (0.0 <= a <= b <= 1.0)
-requires (0 <= k <= |Q|)
+requires problem_requirements(f, g, P, k, a, b, Q)
 
 requires correctSizeInterview(interview, k)
 requires correctQuestionsInterview(interview, k, Q)
 
-ensures postcondition(f, g, P, k, a, b, Q, A, interview, R)
+ensures reveal requires_of_the_postcondition(); postcondition(f, g, P, k, a, b, Q, A, interview, R)
 {
+  
  /* 
   if !correctSizeInterview(interview, k) || !correctQuestionsInterview(interview, k, Q) {
     assert postcondition(f, g, P, k, a, b, Q, A, interview, R) by { reveal postcondition(); }
@@ -31,6 +28,7 @@ ensures postcondition(f, g, P, k, a, b, Q, A, interview, R)
   */
   var paths:set<set<Question>> := getPaths(interview, k, Q);
   R := true;
+  
 
   while 0<|paths|
   decreases |paths|
@@ -63,34 +61,29 @@ ensures postcondition(f, g, P, k, a, b, Q, A, interview, R)
 
   assert requires_of_the_postcondition(f, g, P, k, a, b, Q, A, interview, R) by {
     assert (forall path:set<Question> | path in pathsInterview(interview, k, Q) :: path <= Q);
+    reveal requires_of_the_postcondition();
   }
-  assert postcondition(f, g, P, k, a, b, Q, A, interview, R);
+  assert postcondition(f, g, P, k, a, b, Q, A, interview, R) by { reveal postcondition(); }
 }
 
 
-ghost predicate postcondition(f:map<map<Question, Answer>, bool>, g:map<map<Question, Answer>, int>, P:set<Question>, k:int, a:real, b:real, Q:set<Question>, A:set<Answer>, interview:Interview, R:bool)
-requires (forall m | m in f.Keys :: m.Keys == Q)
-requires (f.Keys == g.Keys)
-requires (P <= Q)
-requires (0.0 <= a <= b <= 1.0)
-requires (0 <= k <= |Q|)
+opaque ghost predicate postcondition(f:map<map<Question, Answer>, bool>, g:map<map<Question, Answer>, int>, P:set<Question>, k:int, a:real, b:real, Q:set<Question>, A:set<Answer>, interview:Interview, R:bool)
+requires problem_requirements(f, g, P, k, a, b, Q)
 requires correctSizeInterview(interview, k)
 requires correctQuestionsInterview(interview, k, Q)
 
 requires requires_of_the_postcondition(f, g, P, k, a, b, Q, A, interview, R) //(forall path:set<Question> | path in pathsInterview(interview, k) :: path <= Q)
 {
+  
   R == (forall path:set<Question> | path in pathsInterview(interview, k, Q) :: verification(f, g, P, k, a, b, Q, path))
 }
 
-ghost predicate requires_of_the_postcondition(f:map<map<Question, Answer>, bool>, g:map<map<Question, Answer>, int>, P:set<Question>, k:int, a:real, b:real, Q:set<Question>, A:set<Answer>, interview:Interview, R:bool)
-requires (forall m | m in f.Keys :: m.Keys == Q)
-requires (f.Keys == g.Keys)
-requires (P <= Q)
-requires (0.0 <= a <= b <= 1.0)
-requires (0 <= k <= |Q|)
+opaque ghost predicate requires_of_the_postcondition(f:map<map<Question, Answer>, bool>, g:map<map<Question, Answer>, int>, P:set<Question>, k:int, a:real, b:real, Q:set<Question>, A:set<Answer>, interview:Interview, R:bool)
+requires problem_requirements(f, g, P, k, a, b, Q)
 requires correctSizeInterview(interview, k)
 requires correctQuestionsInterview(interview, k, Q)
 {
+  
   (forall path:set<Question> | path in pathsInterview(interview, k, Q) :: path <= Q)
 }
 
@@ -140,16 +133,14 @@ ensures R == pathsInterview(interview, k, Q)
     invariant forall path:set<Question> | path in R :: path <= Q
     invariant R == union (set c:Interview | c in (children' - children) :: pathsInterviewPlusElement(c, k-1, interview.Key, Q))
   {
-
     var child:Interview :| child in children;
     var subsets:set<set<Question>> := getPaths(child, k-1, Q) by {
       subinterviewsSmaller(interview, k);
       assert forall child:Interview | child in interview.Children.Values :: correctSizeInterview(child, k-1);
       assert child in interview.Children.Values;
     }
-    //ghost var prev_children:set<Interview> := children;
+
     R, children := getPaths_body_loop(interview, k, Q, R, children, children', child, subsets);
-    //assert |prev_children| == |children| + 1;
   }
 
   assert R == union (set child:Interview | child in children' :: pathsInterviewPlusElement(child, k-1, interview.Key, Q)) by {
@@ -380,7 +371,7 @@ ensures union(set c:Interview | c in (children' - children) :: pathsInterviewPlu
     (f:map<map<Question, Answer>, bool>, g:map<map<Question, Answer>, int>, P:set<Question>, k:int, a:real, b:real, Q:set<Question>, questionsToVerify:set<Question>)
     returns (R:bool)
   
-  requires problem_requirements(f, g, P, k, a, b, Q, questionsToVerify)
+  requires problem_requirements_path(f, g, P, k, a, b, Q, questionsToVerify)
   ensures R == verification(f, g, P, k, a, b, Q, questionsToVerify)
   {
   R := false;
@@ -397,25 +388,25 @@ ensures union(set c:Interview | c in (children' - children) :: pathsInterviewPlu
       assert forall candidate | candidate in candidates :: Q == candidate.Keys by {  }
       assert i == |f.Keys| - |candidates|;
     }
-    assert invariant_loop(f, g, P, Q, candidates, candidates_empty, i) by {
-      reveal invariant_loop();
+    assert auxiliary_invariant_verifyPathCDPC(f, g, P, Q, candidates, candidates_empty, i) by {
+      reveal auxiliary_invariant_verifyPathCDPC();
     }
-    assert verification_loop(f, g, P, k, a, b, Q, questionsToVerify, candidates, R) by { reveal verification_loop();  }
+    assert verification_invariant_verifyPathCDPC(f, g, P, k, a, b, Q, questionsToVerify, candidates, R) by { reveal verification_invariant_verifyPathCDPC();  }
     
     while !candidates_empty 
       decreases |candidates|
-      invariant problem_requirements(f, g, P, k, a, b, Q, questionsToVerify)
-      invariant invariant_loop(f, g, P, Q, candidates, candidates_empty, i)
-      invariant verification_loop(f, g, P, k, a, b, Q, questionsToVerify, candidates, R)
-    {     
+      invariant problem_requirements_path(f, g, P, k, a, b, Q, questionsToVerify)
+      invariant auxiliary_invariant_verifyPathCDPC(f, g, P, Q, candidates, candidates_empty, i)
+      invariant verification_invariant_verifyPathCDPC(f, g, P, k, a, b, Q, questionsToVerify, candidates, R)
+    {
       ghost var candidates_ := candidates;
-      assert candidates <= f.Keys by {reveal invariant_loop();}
+      assert candidates <= f.Keys by {reveal auxiliary_invariant_verifyPathCDPC();}
 
-      candidates, candidates_empty, i, R := body_loop(f, g, P, k, a, b, Q, questionsToVerify, candidates, candidates_empty, i, R);
+      candidates, candidates_empty, i, R := body_verifyPathCDPC(f, g, P, k, a, b, Q, questionsToVerify, candidates, candidates_empty, i, R);
       
       assert |candidates| < |candidates_| by { reveal decreases_body(candidates_, candidates); }
     }
-    assert candidates == {} by {reveal invariant_loop();}
+    assert candidates == {} by {reveal auxiliary_invariant_verifyPathCDPC();}
     allCandidate(f,g,P,k,a,b,Q,questionsToVerify,candidates,R); 
   }
   else {
@@ -429,39 +420,39 @@ ensures union(set c:Interview | c in (children' - children) :: pathsInterviewPlu
 
 
 // Given a set "candidates", takes one candidate out of the set and calculates if the candidates that would have answered in the same way to the questions in "questionsToVerify" are equally fit and that no private information has been inferred
-method body_loop
+method body_verifyPathCDPC
 (f:map<map<Question, Answer>, bool>, g:map<map<Question, Answer>, int>, P:set<Question>, k:int, a:real, b:real, Q:set<Question>, questionsToVerify:set<Question>,
 candidates_:set<map<Question, Answer>>, candidates_empty_:bool, i_:nat, R_:bool)
 returns (candidates:set<map<Question, Answer>>, candidates_empty:bool, i:nat, R:bool)
 
-  requires problem_requirements(f, g, P, k, a, b, Q, questionsToVerify)
+  requires problem_requirements_path(f, g, P, k, a, b, Q, questionsToVerify)
 
   requires !candidates_empty_
-  requires invariant_loop(f, g, P, Q, candidates_, candidates_empty_, i_)
-  requires verification_loop(f, g, P, k, a, b, Q, questionsToVerify, candidates_, R_)
+  requires auxiliary_invariant_verifyPathCDPC(f, g, P, Q, candidates_, candidates_empty_, i_)
+  requires verification_invariant_verifyPathCDPC(f, g, P, k, a, b, Q, questionsToVerify, candidates_, R_)
 
   requires candidates_ <= f.Keys
 
   ensures decreases_body(candidates_, candidates)
-  ensures invariant_loop(f, g, P, Q, candidates, candidates_empty, i)
+  ensures auxiliary_invariant_verifyPathCDPC(f, g, P, Q, candidates, candidates_empty, i)
   
   ensures candidates < candidates_
-  ensures verification_loop(f, g, P, k, a, b, Q, questionsToVerify, candidates, R)
+  ensures verification_invariant_verifyPathCDPC(f, g, P, k, a, b, Q, questionsToVerify, candidates, R)
 {
   candidates := candidates_;
   i := i_;
   candidates_empty := candidates_empty_;
-  label L: assert invariant_loop(f, g, P, Q, candidates_, candidates_empty_, i_);
+  label L: assert auxiliary_invariant_verifyPathCDPC(f, g, P, Q, candidates_, candidates_empty_, i_);
   
   var candidate:map<Question, Answer>;
-  candidate :| candidate in candidates by { reveal invariant_loop(f, g, P, Q, candidates_, candidates_empty_, i_); }
+  candidate :| candidate in candidates by { reveal auxiliary_invariant_verifyPathCDPC(f, g, P, Q, candidates_, candidates_empty_, i_); }
   var person:map<Question, Answer>;
 
   var f':map<map<Question, Answer>, bool>;
   var g':map<map<Question, Answer>, int>;
   
-  f' := those_who_would_answer_the_same(f, candidate, questionsToVerify) by { reveal invariant_loop(f, g, P, Q, candidates_, candidates_empty_, i_);  }
-  g' := those_who_would_answer_the_same(g, candidate, questionsToVerify) by { reveal invariant_loop(f, g, P, Q, candidates_, candidates_empty_, i_);  }
+  f' := those_who_would_answer_the_same(f, candidate, questionsToVerify) by { reveal auxiliary_invariant_verifyPathCDPC(f, g, P, Q, candidates_, candidates_empty_, i_);  }
+  g' := those_who_would_answer_the_same(g, candidate, questionsToVerify) by { reveal auxiliary_invariant_verifyPathCDPC(f, g, P, Q, candidates_, candidates_empty_, i_);  }
   var okFit:bool;
   var okPriv:bool;
   okFit := okFitnessMethod(f');
@@ -481,8 +472,8 @@ returns (candidates:set<map<Question, Answer>>, candidates_empty:bool, i:nat, R:
   ghost var i' := i;
   i := i + 1;
 
-  assert invariant_loop(f, g, P, Q, candidates, candidates_empty, i) by {
-    reveal invariant_loop();
+  assert auxiliary_invariant_verifyPathCDPC(f, g, P, Q, candidates, candidates_empty, i) by {
+    reveal auxiliary_invariant_verifyPathCDPC();
     assert candidates <= f.Keys;
     assert candidates_empty == (candidates == {});
     assert forall candidate | candidate in candidates :: Q == candidate.Keys;
@@ -490,7 +481,7 @@ returns (candidates:set<map<Question, Answer>>, candidates_empty:bool, i:nat, R:
     assert i == |f.Keys| - |candidates|;
   }
   assert decreases_body(candidates_, candidates) by {reveal decreases_body(); }
-  assert verification_loop(f, g, P, k, a, b, Q, questionsToVerify, candidates, R) by
+  assert verification_invariant_verifyPathCDPC(f, g, P, k, a, b, Q, questionsToVerify, candidates, R) by
   { 
     verification_body_lemma(f,g,P,k,a,b,Q,questionsToVerify,candidates_,candidates_empty_,i,R_,f',g',candidates,candidate, okFit,okPriv,R);
   }
@@ -501,17 +492,16 @@ returns (candidates:set<map<Question, Answer>>, candidates_empty:bool, i:nat, R:
 
 
 
-opaque ghost predicate invariant_loop(f:map<map<Question, Answer>, bool>, g:map<map<Question, Answer>, int>, P:set<Question>, Q:set<Question>, candidates:set<map<Question, Answer>>, candidates_empty:bool, i:nat) { //{:opaque}
+opaque ghost predicate auxiliary_invariant_verifyPathCDPC(f:map<map<Question, Answer>, bool>, g:map<map<Question, Answer>, int>, P:set<Question>, Q:set<Question>, candidates:set<map<Question, Answer>>, candidates_empty:bool, i:nat) { //{:opaque}
      (candidates <= f.Keys)
   && (candidates_empty == (candidates == {}))
   && (forall candidate | candidate in candidates :: Q == candidate.Keys)
-  //&& (|candidates| == |candidates_| - 1)
   && (i == |f.Keys| - |candidates|)
 }
-
+/*
 opaque ghost predicate invariant_body_loop(f:map<map<Question, Answer>, bool>, g:map<map<Question, Answer>, int>, P:set<Question>, k:int, a:real, b:real, Q:set<Question>, questionsToVerify:set<Question>,
 candidates_:set<map<Question, Answer>>, candidates_empty_:bool, i_:nat, R_:bool, f':map<map<Question, Answer>, bool>, g':map<map<Question, Answer>, int>, candidates:set<map<Question, Answer>>, candidate:map<Question, Answer>, okFit:bool, okPriv:bool, R:bool)
-requires problem_requirements(f, g, P, k, a, b, Q, questionsToVerify)
+requires problem_requirements_path(f, g, P, k, a, b, Q, questionsToVerify)
 {
  (!candidates_empty_) &&
  (candidates_ <= f.Keys) &&
@@ -523,14 +513,22 @@ requires problem_requirements(f, g, P, k, a, b, Q, questionsToVerify)
  (g' == map person:map<Question, Answer> | person in g.Keys && (forall q:Question | q in questionsToVerify :: person[q] == candidate[q]) :: g[person]) &&
  (okFit == okFitness(f')) &&
  (okPriv == okPrivate(g', P, a, b, Q))
-}
+}*/
 
 
 opaque ghost predicate decreases_body(candidates_:set<map<Question, Answer>>, candidates:set<map<Question, Answer>>) {
   (|candidates| == |candidates_| - 1)
 }
 
-ghost predicate problem_requirements(f:map<map<Question, Answer>, bool>, g:map<map<Question, Answer>, int>, P:set<Question>, k:int, a:real, b:real, Q:set<Question>, questionsToVerify:set<Question>) {
+ghost predicate problem_requirements(f:map<map<Question, Answer>, bool>, g:map<map<Question, Answer>, int>, P:set<Question>, k:int, a:real, b:real, Q:set<Question>) {
+  (forall m | m in f.Keys :: m.Keys == Q) &&
+  (f.Keys == g.Keys) &&
+  (P <= Q) &&
+  (0.0 <= a <= b <= 1.0) &&
+  (0 <= k <= |Q|)
+}
+
+ghost predicate problem_requirements_path(f:map<map<Question, Answer>, bool>, g:map<map<Question, Answer>, int>, P:set<Question>, k:int, a:real, b:real, Q:set<Question>, questionsToVerify:set<Question>) {
   (forall m | m in f.Keys :: m.Keys == Q) &&
   (f.Keys == g.Keys) &&
   (P <= Q) &&
@@ -541,7 +539,7 @@ ghost predicate problem_requirements(f:map<map<Question, Answer>, bool>, g:map<m
 
 
 opaque ghost predicate verification(f:map<map<Question, Answer>, bool>, g:map<map<Question, Answer>, int>, P:set<Question>, k:int, a:real, b:real, Q:set<Question>, questionsToVerify:set<Question>)
-  requires problem_requirements(f, g, P, k, a, b, Q, questionsToVerify)
+  requires problem_requirements_path(f, g, P, k, a, b, Q, questionsToVerify)
 {
   (|questionsToVerify| <= k) &&
   (forall candidate:map<Question, Answer> | candidate in f ::
@@ -554,8 +552,8 @@ opaque ghost predicate verification(f:map<map<Question, Answer>, bool>, g:map<ma
 
 
 lemma allCandidate(f:map<map<Question, Answer>, bool>, g:map<map<Question, Answer>, int>, P:set<Question>, k:int, a:real, b:real, Q:set<Question>, questionsToVerify:set<Question>, candidates:set<map<Question, Answer>>, R:bool)
-requires problem_requirements(f, g, P, k, a, b, Q, questionsToVerify)
-requires verification_loop(f, g, P, k, a, b, Q, questionsToVerify, candidates, R)
+requires problem_requirements_path(f, g, P, k, a, b, Q, questionsToVerify)
+requires verification_invariant_verifyPathCDPC(f, g, P, k, a, b, Q, questionsToVerify, candidates, R)
 requires candidates == {} 
 requires |questionsToVerify| <= k
 ensures R == verification(f, g, P, k, a, b, Q, questionsToVerify)
@@ -583,7 +581,7 @@ ensures R == verification(f, g, P, k, a, b, Q, questionsToVerify)
         var f' := map person:map<Question, Answer> | person in f.Keys && (forall q:Question | q in questionsToVerify :: person[q] == candidate[q]) :: f[person];
         var g' := map person:map<Question, Answer> | person in g.Keys && (forall q:Question | q in questionsToVerify :: person[q] == candidate[q]) :: g[person];
         okFitness(f') && okPrivate(g', P, a, b, Q)
-      )) by { reveal verification_loop(); }
+      )) by { reveal verification_invariant_verifyPathCDPC(); }
     
     assert f.Keys == ((f.Keys - candidates) + candidates) by {
       assert candidates <= f.Keys;
@@ -600,8 +598,8 @@ ensures S == ((S - s) + s)
 }
 
 
-opaque ghost predicate verification_loop(f:map<map<Question, Answer>, bool>, g:map<map<Question, Answer>, int>, P:set<Question>, k:int, a:real, b:real, Q:set<Question>, questionsToVerify:set<Question>, candidates:set<map<Question, Answer>>, R:bool)
-  requires problem_requirements(f, g, P, k, a, b, Q, questionsToVerify)
+opaque ghost predicate verification_invariant_verifyPathCDPC(f:map<map<Question, Answer>, bool>, g:map<map<Question, Answer>, int>, P:set<Question>, k:int, a:real, b:real, Q:set<Question>, questionsToVerify:set<Question>, candidates:set<map<Question, Answer>>, R:bool)
+  requires problem_requirements_path(f, g, P, k, a, b, Q, questionsToVerify)
 {
   R == (forall candidate:map<Question, Answer> | candidate in (f - candidates) :: 
   (
@@ -673,23 +671,143 @@ method okPrivateMethod(g:map<map<Question, Answer>, int>, P:set<Question>, a:rea
   requires 0.0 <= b <= 1.0
   requires a <= b
   ensures R == okPrivate(g, P, a, b, Q)
-/*
+
 {
-  var keys := g.Keys;
-  var nC := 0;
+  var P' := P;
+  R := true;
 
-  while ! (|keys| <= 0)
-    decreases |keys|
-    invariant keys <= g.Keys
-    invariant nC == nCandidates(g, Q)
-  {
-    var key :| key in keys;
-
-    nC := nC + g[key];
-
-    keys := keys - {key};
+  assert R ==
+    forall i:Question | i in (P - P') ::
+      var nC:real := nCandidates(g, Q) as real;
+      var nP:real := nPrivate(g, Q, i, T) as real;
+      if nC == 0.0 then
+        true
+      else
+        a <= nP / nC <= b
+  by {
+    assert (P - P') == {};
   }
+
+  assert R == okPrivate(g, (P - P'), a, b, Q) by {
+    reveal okPrivate();
+
+    assert R ==
+      forall i:Question | i in (P - P') ::
+        var nC:real := nCandidates(g, Q) as real;
+        var nP:real := nPrivate(g, Q, i, T) as real;
+        if nC == 0.0 then
+          true
+        else
+          a <= nP / nC <= b
+    by {
+      assert (P - P') == {};
+    }
+  }
+
+  while P' != {}
+  decreases P'
+  invariant P' <= P
+  invariant R == okPrivate(g, (P - P'), a, b, Q)
+  {
+    ghost var old_P' := P';
+
+    var P'_out;
+    P'_out, R := body_okPrivateMethod(g, P, a, b, Q, P', R) by {
+      reveal preconditions_okPrivateMethod();
+      reveal termination_okPrivateMethod();
+      reveal invariant_entry_okPrivateMethod();
+    }
+    assert R == okPrivate(g, (P - P'_out), a, b, Q) by {
+      reveal invariant_exit_okPrivateMethod();
+    }
+    
+    assert P'_out < P' by {
+      reveal decreases_okPrivateMethod();
+    }
+    P' := P'_out;
+
+    assert R == okPrivate(g, (P - P'), a, b, Q) by {
+      reveal preconditions_okPrivateMethod();
+      reveal termination_okPrivateMethod();
+      reveal invariant_entry_okPrivateMethod();
+    }
+    
+  }
+
 }
+
+
+opaque ghost predicate preconditions_okPrivateMethod(g:map<map<Question, Answer>, int>, P:set<Question>, a:real, b:real, Q:set<Question>, P':set<Question>, R:bool)
+{
+  (forall m | m in g.Keys :: m.Keys == Q)
+  && (P <= Q)
+  && (0.0 <= a <= 1.0)
+  && (0.0 <= b <= 1.0)
+  && (a <= b)
+}
+opaque ghost predicate termination_okPrivateMethod(g:map<map<Question, Answer>, int>, P:set<Question>, a:real, b:real, Q:set<Question>, P':set<Question>, R:bool)
+{
+  P' != {}
+}
+opaque ghost predicate invariant_entry_okPrivateMethod(g:map<map<Question, Answer>, int>, P:set<Question>, a:real, b:real, Q:set<Question>, P':set<Question>, R:bool)
+requires preconditions_okPrivateMethod(g, P, a, b, Q, P', R)
+{
+  reveal preconditions_okPrivateMethod();
+  (P' <= P)
+  && (R ==
+    forall i:Question | i in (P - P') ::
+      var nC:real := nCandidates(g, Q) as real;
+      var nP:real := nPrivate(g, Q, i, T) as real;
+      if nC == 0.0 then
+        true
+      else
+        a <= nP / nC <= b)
+}
+opaque ghost predicate invariant_exit_okPrivateMethod(g:map<map<Question, Answer>, int>, P:set<Question>, a:real, b:real, Q:set<Question>, P':set<Question>, R:bool, P'_out:set<Question>, R_out:bool)
+requires preconditions_okPrivateMethod(g, P, a, b, Q, P', R)
+{
+  reveal preconditions_okPrivateMethod();
+  (P'_out <= P)
+  && (R_out == okPrivate(g, (P - P'_out), a, b, Q))
+}
+opaque ghost predicate decreases_okPrivateMethod(g:map<map<Question, Answer>, int>, P:set<Question>, a:real, b:real, Q:set<Question>, P':set<Question>, R:bool, P'_out:set<Question>, R_out:bool)
+{
+  P'_out < P'
+}
+
+method body_okPrivateMethod(g:map<map<Question, Answer>, int>, P:set<Question>, a:real, b:real, Q:set<Question>, P':set<Question>, R:bool) returns (P'_out:set<Question>, R_out:bool)
+  requires preconditions_okPrivateMethod(g, P, a, b, Q, P', R)
+  requires termination_okPrivateMethod(g, P, a, b, Q, P', R)
+  requires invariant_entry_okPrivateMethod(g, P, a, b, Q, P', R)
+  ensures invariant_exit_okPrivateMethod(g, P, a, b, Q, P', R, P'_out, R_out)
+  ensures decreases_okPrivateMethod(g, P, a, b, Q, P', R, P'_out, R_out)
+{
+
+  P'_out := P';
+  R_out := R;
+
+  var i:Question :| i in P' by { reveal termination_okPrivateMethod(); }
+  var nC:int := nCandidatesMethod(g, Q) by { reveal preconditions_okPrivateMethod(); }
+  var nP:int := nPrivateMethod(g, Q, i, T) by { reveal preconditions_okPrivateMethod(); reveal invariant_entry_okPrivateMethod(); }
+  var real_nC:real := nC as real;
+  var real_nP:real := nP as real;
+
+  if real_nC == 0.0  {}
+  else {
+    R_out := R && (a <= real_nP / real_nC <= b);
+  }
+
+  P'_out := P' - {i};
+
+  assert invariant_exit_okPrivateMethod(g, P, a, b, Q, P', R, P'_out, R_out) by {
+    reveal preconditions_okPrivateMethod();
+    reveal termination_okPrivateMethod();
+    reveal invariant_entry_okPrivateMethod();
+    reveal invariant_exit_okPrivateMethod();
+  }
+  assert decreases_okPrivateMethod(g, P, a, b, Q, P', R, P'_out, R_out) by { reveal decreases_okPrivateMethod(); }
+}
+
 
 method nCandidatesMethod(g:map<map<Question, Answer>, int>, Q:set<Question>) returns (r:int)
   requires forall m | m in g.Keys :: m.Keys == Q
@@ -712,9 +830,106 @@ method nCandidatesMethod(g:map<map<Question, Answer>, int>, Q:set<Question>) ret
           (map m:map<Question, Answer> | m in g.Keys && m != c :: g[m]),
           Q
         );
+
+    nCandidatesLemma(g, Q);
   }
 }
-*/
+
+method nPrivateMethod(g:map<map<Question, Answer>, int>, Q:set<Question>, privateQuestion:Question, selectedAnswer:Answer) returns (r:int)
+requires forall m | m in g.Keys :: m.Keys == Q
+requires privateQuestion in Q
+  ensures r == nPrivate(g, Q, privateQuestion, selectedAnswer)
+{
+  if g.Keys == {} {
+    r := 0;
+    assert r == nPrivate(g, Q, privateQuestion, selectedAnswer);
+  }
+  else {
+    var c:map<Question, Answer> :| c in g.Keys;
+    r := nPrivateMethod(
+      (map m:map<Question, Answer> | m in g.Keys && m != c :: g[m]),
+      Q,
+      privateQuestion,
+      selectedAnswer
+    );
+    r := r + (if c[privateQuestion] == selectedAnswer then g[c] else 0);
+
+    assert var c:map<Question, Answer> := Pick(g.Keys);
+        nPrivate(g, Q, privateQuestion, selectedAnswer) == (if c[privateQuestion] == selectedAnswer then g[c] else 0) + nPrivate(
+      (map m:map<Question, Answer> | m in g.Keys && m != c :: g[m]),
+      Q,
+      privateQuestion,
+      selectedAnswer
+    );
+
+    nPrivateLemma(g, Q, privateQuestion, selectedAnswer);
+  }
+}
+
+lemma nCandidatesLemma(g:map<map<Question, Answer>, int>, Q:set<Question>)
+//decreases |g.Keys|
+requires forall m | m in g.Keys :: m.Keys == Q
+ensures forall c:map<Question, Answer> | c in g.Keys ::
+  nCandidates(g, Q) == g[c] + nCandidates(
+    (map m:map<Question, Answer> | m in g.Keys && m != c :: g[m]),
+    Q
+  )
+{
+  if g.Keys == {} {}
+  else {
+    
+    assert var c:map<Question, Answer> := Pick(g.Keys);
+      nCandidates(g, Q) == g[c] + nCandidates(
+        (map m:map<Question, Answer> | m in g.Keys && m != c :: g[m]),
+        Q
+      );
+
+    assume false;
+
+    assert var c:map<Question, Answer> :| c in g.Keys;
+      nCandidates(g, Q) == g[c] + nCandidates(
+        (map m:map<Question, Answer> | m in g.Keys && m != c :: g[m]),
+        Q
+      );  
+    
+    forall c:map<Question, Answer> | c in g.Keys
+      ensures nCandidates(g, Q) == g[c] + nCandidates(
+          (map m:map<Question, Answer> | m in g.Keys && m != c :: g[m]),
+          Q
+        )
+    {
+    }
+    
+  }
+}
+
+lemma nPrivateLemma(g:map<map<Question, Answer>, int>, Q:set<Question>, privateQuestion:Question, selectedAnswer:Answer)
+//decreases |g.Keys|
+requires forall m | m in g.Keys :: m.Keys == Q
+requires privateQuestion in Q
+ensures forall c:map<Question, Answer> | c in g.Keys ::
+  nPrivate(g, Q, privateQuestion, selectedAnswer) == (if c[privateQuestion] == selectedAnswer then g[c] else 0) + nPrivate(
+    (map m:map<Question, Answer> | m in g.Keys && m != c :: g[m]),
+    Q,
+    privateQuestion,
+    selectedAnswer
+  )
+{
+  if g.Keys == {} {}
+  else {
+    assert var c:map<Question, Answer> := Pick(g.Keys);
+      nPrivate(g, Q, privateQuestion, selectedAnswer) == (if c[privateQuestion] == selectedAnswer then g[c] else 0) + nPrivate(
+      (map m:map<Question, Answer> | m in g.Keys && m != c :: g[m]),
+      Q,
+      privateQuestion,
+      selectedAnswer
+    );
+    assume false;
+  }
+}
+
+
+
 
 
 lemma basic_math(i:nat, a:nat)
@@ -742,7 +957,7 @@ lemma smallerSetLessCardinality<T>(A:set<T>, B:set<T>)
 
 lemma and_identity(f:map<map<Question, Answer>, bool>, g:map<map<Question, Answer>, int>, P:set<Question>, k:int, a:real, b:real, Q:set<Question>, questionsToVerify:set<Question>)
 requires (|questionsToVerify| <= k)
-requires problem_requirements(f, g, P, k, a, b, Q, questionsToVerify)
+requires problem_requirements_path(f, g, P, k, a, b, Q, questionsToVerify)
 
 ensures 
   ((|questionsToVerify| <= k) &&
@@ -765,19 +980,19 @@ ensures
 
 
 lemma verification_loop_recover(f:map<map<Question, Answer>, bool>, g:map<map<Question, Answer>, int>, P:set<Question>, k:int, a:real, b:real, Q:set<Question>, questionsToVerify:set<Question>, candidates:set<map<Question, Answer>>, R:bool)
-requires problem_requirements(f, g, P, k, a, b, Q, questionsToVerify)
+requires problem_requirements_path(f, g, P, k, a, b, Q, questionsToVerify)
 requires R == (forall candidate:map<Question, Answer> | candidate in (f - candidates) ::
     (
       var f' := map person:map<Question, Answer> | person in f.Keys && (forall q:Question | q in questionsToVerify :: person[q] == candidate[q]) :: f[person];
       var g' := map person:map<Question, Answer> | person in g.Keys && (forall q:Question | q in questionsToVerify :: person[q] == candidate[q]) :: g[person];
       okFitness(f') && okPrivate(g', P, a, b, Q)
     ))
-ensures verification_loop(f, g, P, k, a, b, Q, questionsToVerify, candidates,R)
-{reveal verification_loop();}
+ensures verification_invariant_verifyPathCDPC(f, g, P, k, a, b, Q, questionsToVerify, candidates,R)
+{reveal verification_invariant_verifyPathCDPC();}
 
 lemma verification_body_lemma(f:map<map<Question, Answer>, bool>, g:map<map<Question, Answer>, int>, P:set<Question>, k:int, a:real, b:real, Q:set<Question>, questionsToVerify:set<Question>,
 candidates_:set<map<Question, Answer>>, candidates_empty_:bool, i_:nat, R_:bool, f':map<map<Question, Answer>, bool>, g':map<map<Question, Answer>, int>, candidates:set<map<Question, Answer>>, candidate:map<Question, Answer>, okFit:bool, okPriv:bool, R:bool)
-requires problem_requirements(f, g, P, k, a, b, Q, questionsToVerify)
+requires problem_requirements_path(f, g, P, k, a, b, Q, questionsToVerify)
 
 requires !candidates_empty_
 requires candidates_ <= f.Keys
@@ -790,10 +1005,10 @@ requires  g' == map person:map<Question, Answer> | person in g.Keys && (forall q
 requires okFit == okFitness(f')
 requires okPriv == okPrivate(g', P, a, b, Q)
 
-requires verification_loop(f, g, P, k, a, b, Q, questionsToVerify, candidates_,R_)
+requires verification_invariant_verifyPathCDPC(f, g, P, k, a, b, Q, questionsToVerify, candidates_,R_)
 requires R == (R_ && okFit && okPriv)
 
-ensures verification_loop(f, g, P, k, a, b, Q, questionsToVerify, candidates,R)
+ensures verification_invariant_verifyPathCDPC(f, g, P, k, a, b, Q, questionsToVerify, candidates,R)
 {
   // Hipótesis 
   assert 
@@ -802,17 +1017,17 @@ ensures verification_loop(f, g, P, k, a, b, Q, questionsToVerify, candidates,R)
       var f' := map person:map<Question, Answer> | person in f.Keys && (forall q:Question | q in questionsToVerify :: person[q] == candidate[q]) :: f[person];
       var g' := map person:map<Question, Answer> | person in g.Keys && (forall q:Question | q in questionsToVerify :: person[q] == candidate[q]) :: g[person];
       okFitness(f') && okPrivate(g', P, a, b, Q)
-    )) by { reveal verification_loop(); }
+    )) by { reveal verification_invariant_verifyPathCDPC(); }
 
 
   // Este lema demuestra que se cumple que el cuerpo del bucle es correcto. Es decir, demuestra que los cambios que han ocurrido desde el inicio del cuerpo (desde el valor anterior de R; R_) han tenido el efecto deseado
   start_of_loop_values_match_with_end_of_loop_values_body_lemma(f, g, P, k, a, b, Q, questionsToVerify, candidates_, candidates_empty_, i_, R_, f', g', candidates, candidate, okFit, okPriv, R) by {
-    reveal invariant_body_loop();
+    //reveal invariant_body_loop();
   }
 
 
   assert (f.Keys - candidates) == (f.Keys - candidates_) + (candidates_ - candidates) by {
-    reveal invariant_body_loop();
+    //reveal invariant_body_loop();
     assert candidates == candidates_ - {candidate};
     assert (candidates_ - candidates) == {candidate};
     assert (f.Keys - candidates) == (f.Keys - candidates_) + {candidate};
@@ -880,7 +1095,7 @@ ensures verification_loop(f, g, P, k, a, b, Q, questionsToVerify, candidates,R)
 
 lemma forall_of_two_sets_equals_forall_of_combined_sets_body_lemma(f:map<map<Question, Answer>, bool>, g:map<map<Question, Answer>, int>, P:set<Question>, k:int, a:real, b:real, Q:set<Question>, questionsToVerify:set<Question>,
 candidates_:set<map<Question, Answer>>, candidates_empty_:bool, i_:nat, R_:bool, f':map<map<Question, Answer>, bool>, g':map<map<Question, Answer>, int>, candidates:set<map<Question, Answer>>, candidate:map<Question, Answer>, okFit:bool, okPriv:bool, R:bool)
-requires problem_requirements(f, g, P, k, a, b, Q, questionsToVerify)
+requires problem_requirements_path(f, g, P, k, a, b, Q, questionsToVerify)
 requires (f.Keys - candidates) == (f.Keys - candidates_) + (candidates_ - candidates)
 ensures
   ((forall candidate:map<Question, Answer> | candidate in (f.Keys - candidates_) :: 
@@ -934,11 +1149,11 @@ ensures
 
 lemma start_of_loop_values_match_with_end_of_loop_values_body_lemma(f:map<map<Question, Answer>, bool>, g:map<map<Question, Answer>, int>, P:set<Question>, k:int, a:real, b:real, Q:set<Question>, questionsToVerify:set<Question>,
 candidates_:set<map<Question, Answer>>, candidates_empty_:bool, i_:nat, R_:bool, f':map<map<Question, Answer>, bool>, g':map<map<Question, Answer>, int>, candidates:set<map<Question, Answer>>, candidate:map<Question, Answer>, okFit:bool, okPriv:bool, R:bool)
-requires problem_requirements(f, g, P, k, a, b, Q, questionsToVerify)
+requires problem_requirements_path(f, g, P, k, a, b, Q, questionsToVerify)
 
 requires !candidates_empty_
 requires candidates_ <= f.Keys
-//requires invariant_loop(f, g, P, Q, candidates_, candidates_empty_, i_)
+//requires auxiliary_invariant_verifyPathCDPC(f, g, P, Q, candidates_, candidates_empty_, i_)
 
 requires candidate in candidates_
 requires candidates <= candidates_
@@ -948,7 +1163,7 @@ requires  f' == map person:map<Question, Answer> | person in f.Keys && (forall q
 requires  g' == map person:map<Question, Answer> | person in g.Keys && (forall q:Question | q in questionsToVerify :: person[q] == candidate[q]) :: g[person]
 requires okFit == okFitness(f')
 requires okPriv == okPrivate(g', P, a, b, Q)
-requires verification_loop(f, g, P, k, a, b, Q, questionsToVerify, candidates_,R_)
+requires verification_invariant_verifyPathCDPC(f, g, P, k, a, b, Q, questionsToVerify, candidates_,R_)
 requires R == (R_ && okFit && okPriv)
 
 ensures R == (R_ && (forall candidate:map<Question, Answer> | candidate in (candidates_ - candidates) ::
@@ -994,7 +1209,7 @@ ensures R == (R_ && (forall candidate:map<Question, Answer> | candidate in (cand
     okFitness(f') && okPrivate(g', P, a, b, Q))
     ==
     (okFit && okPriv) by {
-        reveal invariant_loop(f, g, P, Q, candidates_, candidates_empty_, i_);
+        reveal auxiliary_invariant_verifyPathCDPC(f, g, P, Q, candidates_, candidates_empty_, i_);
 
       assert f' == map person:map<Question, Answer> | person in f.Keys && (forall q:Question | q in questionsToVerify :: person[q] == candidate[q]) :: f[person];
       assert g' == map person:map<Question, Answer> | person in g.Keys && (forall q:Question | q in questionsToVerify :: person[q] == candidate[q]) :: g[person];
@@ -1033,6 +1248,178 @@ lemma if_contained_then_smaller<A, B>(f':map<A, B>, f:map<A, B>)
     }
   }
 
+
+
+lemma lemma_equal_definition(f:map<map<Question, Answer>, bool>, g:map<map<Question, Answer>, int>, P:set<Question>, k:int, a:real, b:real, Q:set<Question>, A:set<Answer>, interview:Interview, R:bool)
+requires problem_requirements(f, g, P, k, a, b, Q)
+requires correctSizeInterview(interview, k)
+requires correctQuestionsInterview(interview, k, Q)
+requires requires_of_the_postcondition(f, g, P, k, a, b, Q, A, interview, R)    //(forall path:set<Question> | path in pathsInterview(interview, k) :: path <= Q)
+requires postcondition(f, g, P, k, a, b, Q, A, interview, R)
+ensures R == CDPCLim(f, g, P, k, a, b, Q)
+{
+  assert R == (forall path:set<Question> | path in pathsInterview(interview, k, Q) :: verification(f, g, P, k, a, b, Q, path)) by { reveal postcondition();  }
+
+  reveal verification();
+  
+  assert R ==
+    (forall path:set<Question> | path in pathsInterview(interview, k, Q) ::
+      ((|path| <= k) &&
+      (forall candidate:map<Question, Answer> | candidate in f ::
+      (
+        var f' := map person:map<Question, Answer> | person in f.Keys && (forall q:Question | q in path :: person[q] == candidate[q]) :: f[person];
+        var g' := map person:map<Question, Answer> | person in g.Keys && (forall q:Question | q in path :: person[q] == candidate[q]) :: g[person];
+        okFitness(f') && okPrivate(g', P, a, b, Q)
+      )))
+    );
+
+
+
+  assert R == CDPCLim(f, g, P, k, a, b, Q)
+  by {
+
+    assert R == (forall path:set<Question> | path in pathsInterview(interview, k, Q) :: 
+      ((|path| <= k) &&
+      (forall candidate:map<Question, Answer> | candidate in f ::
+      (
+        var f' := map person:map<Question, Answer> | person in f.Keys && (forall q:Question | q in path :: person[q] == candidate[q]) :: f[person];
+        var g' := map person:map<Question, Answer> | person in g.Keys && (forall q:Question | q in path :: person[q] == candidate[q]) :: g[person];
+        okFitness(f') && okPrivate(g', P, a, b, Q)
+      ))))
+    by {
+      assert postcondition(f, g, P, k, a, b, Q, A, interview, R);
+
+      assert R == (forall path:set<Question> | path in pathsInterview(interview, k, Q) :: verification(f, g, P, k, a, b, Q, path));
+
+      assert (forall path:set<Question> | path in pathsInterview(interview, k, Q) :: verification(f, g, P, k, a, b, Q, path)) ==
+              (forall path:set<Question> | path in pathsInterview(interview, k, Q) :: 
+              ((|path| <= k) &&
+              (forall candidate:map<Question, Answer> | candidate in f ::
+              (
+                var f' := map person:map<Question, Answer> | person in f.Keys && (forall q:Question | q in path :: person[q] == candidate[q]) :: f[person];
+                var g' := map person:map<Question, Answer> | person in g.Keys && (forall q:Question | q in path :: person[q] == candidate[q]) :: g[person];
+                okFitness(f') && okPrivate(g', P, a, b, Q)
+              ))));
+    }
+
+
+    assert R == (okPrivate(g, P, a, b, Q) &&
+      if k == 0 then
+        okFitness(f)
+      else
+        okFitness(f) ||
+        exists i:Question | i in Q ::
+          forall o:Answer | o in (set m:map<Question, Answer> | m in f.Keys :: m[i]) ::
+            CDPCLim(
+              restrictMap(f, i, o),
+              restrictMap(g, i, o),
+              P, k - 1, a, b, Q
+            ))
+    by {
+      assert R == (forall path:set<Question> | path in pathsInterview(interview, k, Q) :: 
+        ((|path| <= k) &&
+        (forall candidate:map<Question, Answer> | candidate in f ::
+        (
+          var f' := map person:map<Question, Answer> | person in f.Keys && (forall q:Question | q in path :: person[q] == candidate[q]) :: f[person];
+          var g' := map person:map<Question, Answer> | person in g.Keys && (forall q:Question | q in path :: person[q] == candidate[q]) :: g[person];
+          okFitness(f') && okPrivate(g', P, a, b, Q)
+        ))));
+      lemma_equals_aux(f, g, P, k, a, b, Q, A, interview, R);
+      assume false;
+    }
+    
+    assert
+      CDPCLim(f, g, P, k, a, b, Q)
+      ==
+      (okPrivate(g, P, a, b, Q) &&
+      if k == 0 then
+        okFitness(f)
+      else
+        okFitness(f) ||
+        exists i:Question | i in Q ::
+          forall o:Answer | o in (set m:map<Question, Answer> | m in f.Keys :: m[i]) ::
+            CDPCLim(
+              restrictMap(f, i, o),
+              restrictMap(g, i, o),
+              P, k - 1, a, b, Q
+            ))
+      by {
+        
+        //reveal CDPCLim();
+        assert problem_requirements(f, g, P, k, a, b, Q);
+        assert forall m | m in g.Keys :: m.Keys == Q;
+        assert f.Keys == g.Keys;
+        assert P <= Q;
+        assert 0.0 <= a <= b <= 1.0;
+        assert 0 <= k <= |Q|;
+        lemma_unwrap_CDPCLim(f, g, P, k, a, b, Q);
+
+        assume false;
+      }
+
+    assert R == CDPCLim(f, g, P, k, a, b, Q);
+
+    assume false;
+  }
+
+}
+
+
+
+lemma lemma_unwrap_CDPCLim(f:map<map<Question, Answer>, bool>, g:map<map<Question, Answer>, int>, P:set<Question>, k:int, a:real, b:real, Q:set<Question>)
+  requires problem_requirements(f, g, P, k, a, b, Q)
+  ensures
+    CDPCLim(f, g, P, k, a, b, Q)
+    ==
+    (okPrivate(g, P, a, b, Q) &&
+    if k == 0 then
+      okFitness(f)
+    else
+      okFitness(f) ||
+      exists i:Question | i in Q ::
+        forall o:Answer | o in (set m:map<Question, Answer> | m in f.Keys :: m[i]) ::
+          CDPCLim(
+            restrictMap(f, i, o),
+            restrictMap(g, i, o),
+            P, k - 1, a, b, Q
+          ))
+{
+  reveal CDPCLim();
+  assume false;
+}
+
+
+lemma lemma_equals_aux(f:map<map<Question, Answer>, bool>, g:map<map<Question, Answer>, int>, P:set<Question>, k:int, a:real, b:real, Q:set<Question>, A:set<Answer>, interview:Interview, R:bool)
+requires problem_requirements(f, g, P, k, a, b, Q)
+requires correctSizeInterview(interview, k)
+requires correctQuestionsInterview(interview, k, Q)
+requires requires_of_the_postcondition(f, g, P, k, a, b, Q, A, interview, R)
+requires postcondition(f, g, P, k, a, b, Q, A, interview, R)
+ensures
+  (forall path:set<Question> | path in pathsInterview(interview, k, Q) :: 
+    ((|path| <= k) &&
+    (forall candidate:map<Question, Answer> | candidate in f ::
+    (
+      var f' := map person:map<Question, Answer> | person in f.Keys && (forall q:Question | q in path :: person[q] == candidate[q]) :: f[person];
+      var g' := map person:map<Question, Answer> | person in g.Keys && (forall q:Question | q in path :: person[q] == candidate[q]) :: g[person];
+      okFitness(f') && okPrivate(g', P, a, b, Q)
+    ))))
+  ==
+  (okPrivate(g, P, a, b, Q) &&
+    if k == 0 then
+      okFitness(f)
+    else
+      okFitness(f) ||
+      exists i:Question | i in Q ::
+        forall o:Answer | o in (set m:map<Question, Answer> | m in f.Keys :: m[i]) ::
+          CDPCLim(
+            restrictMap(f, i, o),
+            restrictMap(g, i, o),
+            P, k - 1, a, b, Q
+          ))
+{
+  assume false;
+}
 
 
 }
